@prefix : <http://www.semanticweb.org/kiki/ontologies/2024/3/Global_Airline_Satisfaction_Framework#> .
@prefix owl: <http://www.w3.org/2002/07/owl#> .
@prefix rdf: <http://www.w3.org/1999/02/22-rdf-syntax-ns#> .
@prefix xml: <http://www.w3.org/XML/1998/namespace> .
@prefix xsd: <http://www.w3.org/2001/XMLSchema#> .
@prefix rdfs: <http://www.w3.org/2000/01/rdf-schema#> .
@base <http://www.semanticweb.org/kiki/ontologies/2024/3/Global_Airline_Satisfaction_Framework#> .

<http://www.semanticweb.org/kiki/ontologies/2024/3/Global_Airline_Satisfaction_Framework> rdf:type owl:Ontology ;
                                                                                           rdfs:comment "A structured framework designed to aggregate and analyze customer satisfaction metrics from worldwide airline services, emphasizing the evaluation of in-flight amenities, seating arrangements, and the effectiveness of customer service." ;
                                                                                           rdfs:label "Global Airline Satisfaction Framework" .

#################################################################
#    Annotation properties
#################################################################

###  http://swrl.stanford.edu/ontologies/3.3/swrla.owl#isRuleEnabled
<http://swrl.stanford.edu/ontologies/3.3/swrla.owl#isRuleEnabled> rdf:type owl:AnnotationProperty .


###  http://www.semanticweb.org/kiki/ontologies/2024/3/Global_Airline_Satisfaction_Framework#sameAs
:sameAs rdf:type owl:AnnotationProperty .


#################################################################
#    Object Properties
#################################################################

###  http://www.semanticweb.org/kiki/ontologies/2024/3/Global_Airline_Satisfaction_Framework#bookedOnAirline
:bookedOnAirline rdf:type owl:ObjectProperty ;
                 rdfs:comment "Relates an airline to the airports at which it operates." ;
                 rdfs:label "located_at_airport" .


###  http://www.semanticweb.org/kiki/ontologies/2024/3/Global_Airline_Satisfaction_Framework#hasLoyaltyPoints
:hasLoyaltyPoints rdf:type owl:ObjectProperty ;
                  rdfs:domain :Passenger ;
                  rdfs:range :Loyalty_Rewards ;
                  rdfs:comment "Match a Passenger with their loyalty points" ;
                  rdfs:label "hasLoyaltyPoints" .


###  http://www.semanticweb.org/kiki/ontologies/2024/3/Global_Airline_Satisfaction_Framework#locatedAtAirport
:locatedAtAirport rdf:type owl:ObjectProperty ,
                           owl:FunctionalProperty ;
                  rdfs:comment "Relates a passenger to the airline they have booked for travel." ;
                  rdfs:label "booked_on_airline" .


#################################################################
#    Data properties
#################################################################

###  http://www.semanticweb.org/kiki/ontologies/2024/3/Global_Airline_Satisfaction_Framework#bookedOnFlight
:bookedOnFlight rdf:type owl:DatatypeProperty ;
                rdfs:domain :Flight_Schedule ;
                rdfs:range xsd:boolean ;
                rdfs:comment "booked On Flight" ;
                rdfs:label "bookedOnFlight" .


###  http://www.semanticweb.org/kiki/ontologies/2024/3/Global_Airline_Satisfaction_Framework#departureDate
:departureDate rdf:type owl:DatatypeProperty ;
               rdfs:domain :Flight_Schedule ;
               rdfs:range xsd:dateTime ;
               rdfs:comment "The scheduled date of departure for the flight" ;
               rdfs:label "departureDate" .


###  http://www.semanticweb.org/kiki/ontologies/2024/3/Global_Airline_Satisfaction_Framework#email
:email rdf:type owl:DatatypeProperty ;
       rdfs:domain :Passenger ;
       rdfs:range xsd:string ;
       rdfs:comment "The email address of the passenger for receiving travel confirmations and updates." ;
       rdfs:label "email" .


###  http://www.semanticweb.org/kiki/ontologies/2024/3/Global_Airline_Satisfaction_Framework#hasBoardingStatus
:hasBoardingStatus rdf:type owl:DatatypeProperty ;
                   rdfs:domain :Passenger ;
                   rdfs:range xsd:boolean ;
                   rdfs:comment "Matches a Passenger with his boarding status" ;
                   rdfs:label "hasBoardingStatus" .


###  http://www.semanticweb.org/kiki/ontologies/2024/3/Global_Airline_Satisfaction_Framework#hasSatisfactionRating
:hasSatisfactionRating rdf:type owl:DatatypeProperty ;
                       rdfs:domain :Passenger ;
                       rdfs:range xsd:int ;
                       rdfs:comment "hasSatisfactionRating" ;
                       rdfs:label "hasSatisfactionRating" .


###  http://www.semanticweb.org/kiki/ontologies/2024/3/Global_Airline_Satisfaction_Framework#isDelayed
:isDelayed rdf:type owl:DatatypeProperty ;
           rdfs:domain :Flight_Schedule ;
           rdfs:range xsd:boolean ;
           rdfs:comment "indicates if it is delayed" ;
           rdfs:label "isDelayed" .


###  http://www.semanticweb.org/kiki/ontologies/2024/3/Global_Airline_Satisfaction_Framework#isNotifiedOfDelay
:isNotifiedOfDelay rdf:type owl:DatatypeProperty ;
                   rdfs:domain :Passenger ;
                   rdfs:range xsd:boolean ;
                   rdfs:comment "indicates whether the passenger has been notified of the delay" ;
                   rdfs:label "isNotifiedOfDelay" .


###  http://www.semanticweb.org/kiki/ontologies/2024/3/Global_Airline_Satisfaction_Framework#location
:location rdf:type owl:DatatypeProperty ;
          rdfs:subPropertyOf owl:topDataProperty ;
          rdfs:domain :Airport ;
          rdfs:range xsd:string ;
          rdfs:comment "different locations" ;
          rdfs:label "location" .


###  http://www.semanticweb.org/kiki/ontologies/2024/3/Global_Airline_Satisfaction_Framework#loyaltyPoints
:loyaltyPoints rdf:type owl:DatatypeProperty ;
               rdfs:comment "loyalty Points" ;
               rdfs:label "loyalty_Points" .


###  http://www.semanticweb.org/kiki/ontologies/2024/3/Global_Airline_Satisfaction_Framework#name
:name rdf:type owl:DatatypeProperty ;
      rdfs:domain :Airline ;
      rdfs:range xsd:string ;
      rdfs:comment "type of name" ;
      rdfs:label "name" .


###  http://www.semanticweb.org/kiki/ontologies/2024/3/Global_Airline_Satisfaction_Framework#offeredDiscount
:offeredDiscount rdf:type owl:DatatypeProperty ;
                 rdfs:domain :Passenger ;
                 rdfs:range xsd:boolean ;
                 rdfs:comment "offered Discount" ,
                              "offeredDiscount" .


###  http://www.semanticweb.org/kiki/ontologies/2024/3/Global_Airline_Satisfaction_Framework#policyDescription
:policyDescription rdf:type owl:DatatypeProperty ,
                            owl:FunctionalProperty ;
                   rdfs:domain :Airline_Policies ;
                   rdfs:range xsd:string ;
                   rdfs:comment "policyDescription" ;
                   rdfs:label "policyDescription" .


#################################################################
#    Classes
#################################################################

###  http://www.semanticweb.org/kiki/ontologies/2024/3/Global_Airline_Satisfaction_Framework#Actual_Time
:Actual_Time rdf:type owl:Class ;
             rdfs:subClassOf :Flight_Schedule ;
             rdfs:comment "The real-time at which a flight actually departs or arrives, which may differ from the scheduled time due to various factors." ;
             rdfs:label "Actual_Time" .


###  http://www.semanticweb.org/kiki/ontologies/2024/3/Global_Airline_Satisfaction_Framework#Airline
:Airline rdf:type owl:Class ;
         :sameAs "http://dbpedia.org/resource/Airline" ;
         rdfs:comment "Represents an airline company that provides air transport services for traveling passengers" ;
         rdfs:label "Airline" .


###  http://www.semanticweb.org/kiki/ontologies/2024/3/Global_Airline_Satisfaction_Framework#Airline_Policies
:Airline_Policies rdf:type owl:Class ;
                  rdfs:comment "Encompasses various policies set by the airline regarding passenger handling and service provision." ;
                  rdfs:label "Airline_Policies" .


###  http://www.semanticweb.org/kiki/ontologies/2024/3/Global_Airline_Satisfaction_Framework#Airport
:Airport rdf:type owl:Class ;
         :sameAs "http://dbpedia.org/resource/Airport." ;
         rdfs:comment "Represents an airport, which is a complex comprising runways and buildings for the arrival and departure of aircraft, including facilities for passengers." ;
         rdfs:label "Airport" .


###  http://www.semanticweb.org/kiki/ontologies/2024/3/Global_Airline_Satisfaction_Framework#Airport_Infrastructure
:Airport_Infrastructure rdf:type owl:Class ;
                        rdfs:comment "Physical and organizational structures and facilities for the operation of airports." ;
                        rdfs:label "Airport_Infrastructure" .


###  http://www.semanticweb.org/kiki/ontologies/2024/3/Global_Airline_Satisfaction_Framework#Baggage
:Baggage rdf:type owl:Class ;
         rdfs:comment "Baggage" ,
                      "Covers all aspects of baggage handling and policies for passengers' luggage" .


###  http://www.semanticweb.org/kiki/ontologies/2024/3/Global_Airline_Satisfaction_Framework#Boarding_Process
:Boarding_Process rdf:type owl:Class ;
                  rdfs:subClassOf :Cabin_Layout ;
                  rdfs:comment "The process through which passengers are admitted onto their flights at the gate" ;
                  rdfs:label "Boarding_Process" .


###  http://www.semanticweb.org/kiki/ontologies/2024/3/Global_Airline_Satisfaction_Framework#Business
:Business rdf:type owl:Class ;
          rdfs:subClassOf :Travel_Class ;
          rdfs:comment "A class of service that offers enhanced comfort, space, and service compared to economy class" ;
          rdfs:label "Business" .


###  http://www.semanticweb.org/kiki/ontologies/2024/3/Global_Airline_Satisfaction_Framework#Business_Traveler
:Business_Traveler rdf:type owl:Class ;
                   rdfs:subClassOf :Passenger .


###  http://www.semanticweb.org/kiki/ontologies/2024/3/Global_Airline_Satisfaction_Framework#Cabin_Layout
:Cabin_Layout rdf:type owl:Class ;
              rdfs:comment "The arrangement of seats and facilities within the aircraft cabin, which varies by aircraft and airline" ;
              rdfs:label "Cabin_Layout" .


###  http://www.semanticweb.org/kiki/ontologies/2024/3/Global_Airline_Satisfaction_Framework#Cancellation_Policy
:Cancellation_Policy rdf:type owl:Class ;
                     rdfs:subClassOf :Airline_Policies ;
                     rdfs:comment "Guidelines and procedures for cancelling a flight and the associated refunds or penalties." ;
                     rdfs:label "Cancellation_Policy" .


###  http://www.semanticweb.org/kiki/ontologies/2024/3/Global_Airline_Satisfaction_Framework#Cancellations
:Cancellations rdf:type owl:Class ;
               rdfs:subClassOf :Incidents ;
               rdfs:comment "Flights that are not operated as scheduled due to various reasons like weather or operational issues" ;
               rdfs:label "Cancellations" .


###  http://www.semanticweb.org/kiki/ontologies/2024/3/Global_Airline_Satisfaction_Framework#Carbon_Offsetting
:Carbon_Offsetting rdf:type owl:Class ;
                   rdfs:subClassOf :Environmental_Impact ;
                   rdfs:comment "Initiatives that aim to offset carbon emissions produced by flights through various environmental projects." ;
                   rdfs:label "Carbon_Offsetting" .


###  http://www.semanticweb.org/kiki/ontologies/2024/3/Global_Airline_Satisfaction_Framework#Carry-on_Baggage
:Carry-on_Baggage rdf:type owl:Class ;
                  rdfs:subClassOf :Baggage ;
                  rdfs:comment "Refers to the luggage that passengers are allowed to bring into the cabin." ;
                  rdfs:label "Carry-on_Baggage" .


###  http://www.semanticweb.org/kiki/ontologies/2024/3/Global_Airline_Satisfaction_Framework#Casual_Traveler
:Casual_Traveler rdf:type owl:Class ;
                 rdfs:subClassOf :Passenger ;
                 rdfs:comment "A passenger who travels occasionally, not frequently enough to benefit from loyalty programs." ;
                 rdfs:label "Casual_Traveler" .


###  http://www.semanticweb.org/kiki/ontologies/2024/3/Global_Airline_Satisfaction_Framework#Check-In_Process
:Check-In_Process rdf:type owl:Class ;
                  rdfs:comment "The process by which passengers confirm their presence on a flight and possibly choose their seats and print their boarding passes" ;
                  rdfs:label "Check-In_Process" .


###  http://www.semanticweb.org/kiki/ontologies/2024/3/Global_Airline_Satisfaction_Framework#Checked_Baggage
:Checked_Baggage rdf:type owl:Class ;
                 rdfs:subClassOf :Baggage ;
                 rdfs:comment "Refers to the luggage that is transported in the hold of the aircraft." ;
                 rdfs:label "Checked_Baggage" .


###  http://www.semanticweb.org/kiki/ontologies/2024/3/Global_Airline_Satisfaction_Framework#Connectivity_Solutions
:Connectivity_Solutions rdf:type owl:Class ;
                        rdfs:subClassOf :In-Flight_Technology ;
                        rdfs:comment "Solutions that allow passengers to connect to the internet and other communication networks during the flight" ;
                        rdfs:label "Connectivity_Solutions" .


###  http://www.semanticweb.org/kiki/ontologies/2024/3/Global_Airline_Satisfaction_Framework#Crew_Training
:Crew_Training rdf:type owl:Class ;
               rdfs:comment "Programs and courses aimed at training flight and cabin crew to handle operational duties and ensure passenger safety." ;
               rdfs:label "Crew_Training" .


###  http://www.semanticweb.org/kiki/ontologies/2024/3/Global_Airline_Satisfaction_Framework#Customer_Suppor
:Customer_Suppor rdf:type owl:Class ;
                 rdfs:subClassOf :Service ;
                 rdfs:comment "Support services provided by the airline to assist passengers with inquiries, bookings, and issues." ;
                 rdfs:label "Customer_Support" .


###  http://www.semanticweb.org/kiki/ontologies/2024/3/Global_Airline_Satisfaction_Framework#Delays
:Delays rdf:type owl:Class ;
        rdfs:subClassOf :Incidents ;
        rdfs:comment "Occur when a flight does not depart or arrive at its scheduled time" ;
        rdfs:label "Delays" .


###  http://www.semanticweb.org/kiki/ontologies/2024/3/Global_Airline_Satisfaction_Framework#Desk_Check-In
:Desk_Check-In rdf:type owl:Class ;
               rdfs:subClassOf :Check-In_Process ;
               rdfs:comment "A traditional check-in process where passengers interact with airline staff at a check-in desk at the airport." ;
               rdfs:label "Desk_Check-In" .


###  http://www.semanticweb.org/kiki/ontologies/2024/3/Global_Airline_Satisfaction_Framework#Destination_Airport
:Destination_Airport rdf:type owl:Class ;
                     rdfs:subClassOf :Airport ;
                     rdfs:comment "The airport at which a flight arrives." ;
                     rdfs:label "Destination_Airport" .


###  http://www.semanticweb.org/kiki/ontologies/2024/3/Global_Airline_Satisfaction_Framework#Economy
:Economy rdf:type owl:Class ;
         rdfs:subClassOf :Travel_Class ;
         rdfs:comment "The most basic class of service offering standard amenities at the most affordable price" ;
         rdfs:label "Economy" .


###  http://www.semanticweb.org/kiki/ontologies/2024/3/Global_Airline_Satisfaction_Framework#Emergency_Procedures
:Emergency_Procedures rdf:type owl:Class ;
                      rdfs:subClassOf :Safety_Measures ;
                      rdfs:comment "Procedures and protocols in place to handle emergencies such as medical issues, evacuations, or technical failures during a flight." ;
                      rdfs:label "Emergency_Procedures" .


###  http://www.semanticweb.org/kiki/ontologies/2024/3/Global_Airline_Satisfaction_Framework#Entertainment_Systems
:Entertainment_Systems rdf:type owl:Class ;
                       rdfs:subClassOf :In-Flight_Technology ;
                       rdfs:comment "Systems providing audio and video entertainment to passengers during the flight" ;
                       rdfs:label "Entertainment_Systems" .


###  http://www.semanticweb.org/kiki/ontologies/2024/3/Global_Airline_Satisfaction_Framework#Environmental_Impact
:Environmental_Impact rdf:type owl:Class ;
                      rdfs:comment "Concerns the environmental effects associated with airline operations and initiatives to mitigate them" ;
                      rdfs:label "Environmental_Impact" .


###  http://www.semanticweb.org/kiki/ontologies/2024/3/Global_Airline_Satisfaction_Framework#First_Class
:First_Class rdf:type owl:Class ;
             rdfs:subClassOf :Travel_Class ;
             rdfs:comment "The highest class of service providing luxurious accommodations and the highest level of service" ;
             rdfs:label "First_Class" .


###  http://www.semanticweb.org/kiki/ontologies/2024/3/Global_Airline_Satisfaction_Framework#Flight_Information_Systems
:Flight_Information_Systems rdf:type owl:Class ;
                            rdfs:subClassOf :In-Flight_Technology ;
                            rdfs:comment "Systems that provide real-time flight data to passengers, such as altitude, speed, and estimated time of arrival." ;
                            rdfs:label "Flight_Information_Systems" .


###  http://www.semanticweb.org/kiki/ontologies/2024/3/Global_Airline_Satisfaction_Framework#Flight_Schedule
:Flight_Schedule rdf:type owl:Class ;
                 rdfs:comment "Information about the timing of flights, including planned and actual departure and arrival times" ;
                 rdfs:label "Flight_Schedule" .


###  http://www.semanticweb.org/kiki/ontologies/2024/3/Global_Airline_Satisfaction_Framework#Frequent_Flyer
:Frequent_Flyer rdf:type owl:Class ;
                rdfs:subClassOf :Passenger ;
                rdfs:comment "A passenger who travels frequently, often participating in a loyalty program." ;
                rdfs:label "Frequent_Flyer" .


###  http://www.semanticweb.org/kiki/ontologies/2024/3/Global_Airline_Satisfaction_Framework#Fuel_Efficiency_Programs
:Fuel_Efficiency_Programs rdf:type owl:Class ;
                          rdfs:subClassOf :Environmental_Impact ;
                          rdfs:comment "Programs aimed at reducing fuel consumption and increasing the efficiency of aircraft operations." ;
                          rdfs:label "Fuel_Efficiency_Programs" .


###  http://www.semanticweb.org/kiki/ontologies/2024/3/Global_Airline_Satisfaction_Framework#General_Boarding
:General_Boarding rdf:type owl:Class ;
                  rdfs:subClassOf :Boarding_Process ;
                  rdfs:comment "The standard boarding process where passengers are called to board based on their seat assignment or zone" ;
                  rdfs:label "General_Boarding" .


###  http://www.semanticweb.org/kiki/ontologies/2024/3/Global_Airline_Satisfaction_Framework#Ground_Service
:Ground_Service rdf:type owl:Class ;
                rdfs:subClassOf :Service ;
                rdfs:comment "Services provided at the airport before departure or after arrival, including check-in and baggage handling" ;
                rdfs:label "Ground_Service" .


###  http://www.semanticweb.org/kiki/ontologies/2024/3/Global_Airline_Satisfaction_Framework#Ground_Transportation
:Ground_Transportation rdf:type owl:Class ;
                       rdfs:subClassOf :Airport_Infrastructure ;
                       rdfs:comment "Transportation options available to passengers to and from the airport" ;
                       rdfs:label "Ground_Transportation" .


###  http://www.semanticweb.org/kiki/ontologies/2024/3/Global_Airline_Satisfaction_Framework#Health_Advisory
:Health_Advisory rdf:type owl:Class ;
                 rdfs:subClassOf :Passenger_Health_Services ;
                 rdfs:comment "Advice and information provided to passengers regarding health precautions and necessary medical procedures for travel." ;
                 rdfs:label "Health_Advisory" .


###  http://www.semanticweb.org/kiki/ontologies/2024/3/Global_Airline_Satisfaction_Framework#Health_Measures
:Health_Measures rdf:type owl:Class ;
                 rdfs:subClassOf :Safety_Measures ;
                 rdfs:comment "Preventive health and sanitation measures taken to protect passengers, including hygiene protocols and medical screenings" ;
                 rdfs:label "Health_Measures" .


###  http://www.semanticweb.org/kiki/ontologies/2024/3/Global_Airline_Satisfaction_Framework#In-Flight_Service
:In-Flight_Service rdf:type owl:Class ;
                   rdfs:subClassOf :Service .


###  http://www.semanticweb.org/kiki/ontologies/2024/3/Global_Airline_Satisfaction_Framework#In-Flight_Technology
:In-Flight_Technology rdf:type owl:Class ;
                      rdfs:comment "Technology used on board to enhance passenger experience and flight operations." ;
                      rdfs:label "In-Flight_Technology" .


###  http://www.semanticweb.org/kiki/ontologies/2024/3/Global_Airline_Satisfaction_Framework#Incidents
:Incidents rdf:type owl:Class ;
           rdfs:label "Incidents" ,
                      "Represents various disruptions that can occur during airline operations" .


###  http://www.semanticweb.org/kiki/ontologies/2024/3/Global_Airline_Satisfaction_Framework#Kiosk_Check-In
:Kiosk_Check-In rdf:type owl:Class ;
                rdfs:subClassOf :Check-In_Process ;
                rdfs:comment "A self-service check-in process using kiosks at the airport, allowing passengers to check-in, select seats, and print boarding passes" ;
                rdfs:label "Kiosk_Check-In" .


###  http://www.semanticweb.org/kiki/ontologies/2024/3/Global_Airline_Satisfaction_Framework#Leisure_Traveler
:Leisure_Traveler rdf:type owl:Class ;
                  rdfs:subClassOf :Passenger .


###  http://www.semanticweb.org/kiki/ontologies/2024/3/Global_Airline_Satisfaction_Framework#Loyalty_Rewards
:Loyalty_Rewards rdf:type owl:Class ;
                 rdfs:label "Loyalty_Rewards" ,
                            "Programs designed to reward frequent flyers with benefits and privileges." .


###  http://www.semanticweb.org/kiki/ontologies/2024/3/Global_Airline_Satisfaction_Framework#Luggage_Policy
:Luggage_Policy rdf:type owl:Class ;
                rdfs:subClassOf :Airline_Policies ;
                rdfs:comment "Policy regarding the type and amount of luggage that can be carried on board or checked in." ;
                rdfs:label "Luggage_Policy" .


###  http://www.semanticweb.org/kiki/ontologies/2024/3/Global_Airline_Satisfaction_Framework#Meal_Service
:Meal_Service rdf:type owl:Class ;
              rdfs:comment "Covers the different types of meal options available to passengers during a flight." ;
              rdfs:label "Meal_Service" .


###  http://www.semanticweb.org/kiki/ontologies/2024/3/Global_Airline_Satisfaction_Framework#Medical_Kits_on_Board
:Medical_Kits_on_Board rdf:type owl:Class ;
                       rdfs:subClassOf :Passenger_Health_Services ;
                       rdfs:comment "Medical kits available on flights to handle health emergencies and basic medical needs" ;
                       rdfs:label "Medical_Kits_on_Board" .


###  http://www.semanticweb.org/kiki/ontologies/2024/3/Global_Airline_Satisfaction_Framework#Mileage_Accrual
:Mileage_Accrual rdf:type owl:Class ;
                 rdfs:subClassOf :Loyalty_Rewards ;
                 rdfs:comment "he process of earning miles for flights flown and other eligible activities." ;
                 rdfs:label "Mileage_Accrual" .


###  http://www.semanticweb.org/kiki/ontologies/2024/3/Global_Airline_Satisfaction_Framework#Multiple_Class_Configuration
:Multiple_Class_Configuration rdf:type owl:Class ;
                              rdfs:subClassOf :Cabin_Layout ;
                              rdfs:comment "A cabin layout that includes multiple classes of service, such as economy, business, and first class" ;
                              rdfs:label "Multiple_Class_Configuration" .


###  http://www.semanticweb.org/kiki/ontologies/2024/3/Global_Airline_Satisfaction_Framework#Online_Check-In
:Online_Check-In rdf:type owl:Class ;
                 rdfs:subClassOf :Check-In_Process ;
                 rdfs:comment "A process that allows passengers to check-in and print boarding passes online before arriving at the airport" ;
                 rdfs:label "Online Check-In" .


###  http://www.semanticweb.org/kiki/ontologies/2024/3/Global_Airline_Satisfaction_Framework#Origin_Airport
:Origin_Airport rdf:type owl:Class ;
                rdfs:subClassOf :Airport ;
                rdfs:comment "The airport from which a flight departs." ;
                rdfs:label "Origin_Airport" .


###  http://www.semanticweb.org/kiki/ontologies/2024/3/Global_Airline_Satisfaction_Framework#Overbookings
:Overbookings rdf:type owl:Class ;
              rdfs:subClassOf :Incidents ;
              rdfs:comment "Situations where more tickets are sold than available seats on the aircraft." ;
              rdfs:label "Overbookings" .


###  http://www.semanticweb.org/kiki/ontologies/2024/3/Global_Airline_Satisfaction_Framework#Passenger
:Passenger rdf:type owl:Class ;
           owl:equivalentClass [ rdf:type owl:Restriction ;
                                 owl:onProperty :loyaltyPoints ;
                                 owl:minQualifiedCardinality "0"^^xsd:nonNegativeInteger ;
                                 owl:onDataRange xsd:string
                               ] ,
                               [ rdf:type owl:Restriction ;
                                 owl:onProperty :email ;
                                 owl:qualifiedCardinality "1"^^xsd:nonNegativeInteger ;
                                 owl:onDataRange xsd:string
                               ] ;
           rdfs:comment "Represents an individual who travels in an airplane from one location to another" ;
           rdfs:label "Passenger" .


###  http://www.semanticweb.org/kiki/ontologies/2024/3/Global_Airline_Satisfaction_Framework#Passenger_Health_Services
:Passenger_Health_Services rdf:type owl:Class ;
                           rdfs:comment "Services and measures provided to ensure the health and well-being of passengers during flights." ;
                           rdfs:label "Passenger_Health_Services" .


###  http://www.semanticweb.org/kiki/ontologies/2024/3/Global_Airline_Satisfaction_Framework#Pet_Policy
:Pet_Policy rdf:type owl:Class ;
            rdfs:subClassOf :Airline_Policies ;
            rdfs:comment "Rules and regulations concerning the transport of pets on aircraft." ;
            rdfs:label "Pet_Policy" .


###  http://www.semanticweb.org/kiki/ontologies/2024/3/Global_Airline_Satisfaction_Framework#Priority_Boarding
:Priority_Boarding rdf:type owl:Class ;
                   rdfs:subClassOf :Boarding_Process ;
                   rdfs:comment "A boarding process for passengers with priority status, such as first-class passengers or frequent flyers, allowing them earlier access to the plane." ;
                   rdfs:label "Priority_Boarding" .


###  http://www.semanticweb.org/kiki/ontologies/2024/3/Global_Airline_Satisfaction_Framework#Qatar_Airways
:Qatar_Airways rdf:type owl:Class ;
               rdfs:subClassOf :Airline ;
               rdfs:comment "Qatar Airways is a major airline providing international flights, known for its high service quality." ;
               rdfs:label "QatarAirways" .


###  http://www.semanticweb.org/kiki/ontologies/2024/3/Global_Airline_Satisfaction_Framework#Redemption_Options
:Redemption_Options rdf:type owl:Class ;
                    rdfs:subClassOf :Loyalty_Rewards ;
                    rdfs:comment "Various ways in which accumulated miles can be redeemed, such as for flights, upgrades, or other services." ;
                    rdfs:label "Redemption Options" .


###  http://www.semanticweb.org/kiki/ontologies/2024/3/Global_Airline_Satisfaction_Framework#Runway_Systems
:Runway_Systems rdf:type owl:Class ;
                rdfs:subClassOf :Airport_Infrastructure ;
                rdfs:comment "Systems that manage the runways at airports including their maintenance and usage scheduling." ;
                rdfs:label "Runway_Systems" .


###  http://www.semanticweb.org/kiki/ontologies/2024/3/Global_Airline_Satisfaction_Framework#Ryanair
:Ryanair rdf:type owl:Class ;
         rdfs:subClassOf :Airline ;
         rdfs:comment "Ryanair is a budget airline based in Europe, known for its low-cost flight services." ;
         rdfs:label "Ryanair" .


###  http://www.semanticweb.org/kiki/ontologies/2024/3/Global_Airline_Satisfaction_Framework#Safety_Measures
:Safety_Measures rdf:type owl:Class ;
                 rdfs:comment "Encompasses various safety protocols and emergency procedures implemented by the airline to ensure passenger safety" ;
                 rdfs:label "Safety_Measures" .


###  http://www.semanticweb.org/kiki/ontologies/2024/3/Global_Airline_Satisfaction_Framework#Safety_Training
:Safety_Training rdf:type owl:Class ;
                 rdfs:subClassOf :Crew_Training ;
                 rdfs:comment "Training focused on emergency procedures and safety protocols." ;
                 rdfs:label "Safety_Training" .


###  http://www.semanticweb.org/kiki/ontologies/2024/3/Global_Airline_Satisfaction_Framework#Scheduled_Time
:Scheduled_Time rdf:type owl:Class ;
                rdfs:subClassOf :Flight_Schedule ;
                rdfs:comment "The time at which a flight is originally planned to depart or arrive." ;
                rdfs:label "Scheduled_Time" .


###  http://www.semanticweb.org/kiki/ontologies/2024/3/Global_Airline_Satisfaction_Framework#Service
:Service rdf:type owl:Class ;
         rdfs:comment "Represents various types of services provided by the airline, including in-flight and on the ground services" ;
         rdfs:label "Service" .


###  http://www.semanticweb.org/kiki/ontologies/2024/3/Global_Airline_Satisfaction_Framework#Service_Training
:Service_Training rdf:type owl:Class ;
                  rdfs:subClassOf :Crew_Training ;
                  rdfs:comment "Training that equips crew members with skills for superior passenger service." ;
                  rdfs:label "Service_Training" .


###  http://www.semanticweb.org/kiki/ontologies/2024/3/Global_Airline_Satisfaction_Framework#Single_Class_Configuration
:Single_Class_Configuration rdf:type owl:Class ;
                            rdfs:subClassOf :Cabin_Layout ;
                            rdfs:comment "A cabin layout where the entire aircraft is configured with a single class of service." ;
                            rdfs:label "Single_Class_Configuration" .


###  http://www.semanticweb.org/kiki/ontologies/2024/3/Global_Airline_Satisfaction_Framework#Special_Assistance_Services
:Special_Assistance_Services rdf:type owl:Class ;
                             rdfs:subClassOf :Passenger_Health_Services ;
                             rdfs:comment "Services provided to passengers requiring additional health-related assistance, such as those with disabilities or elderly passengers" ;
                             rdfs:label "Special_Assistance_Services" .


###  http://www.semanticweb.org/kiki/ontologies/2024/3/Global_Airline_Satisfaction_Framework#Special_Meal
:Special_Meal rdf:type owl:Class ;
              rdfs:subClassOf :Meal_Service ;
              rdfs:comment "Meals designed to meet specific dietary requirements or preferences, such as vegetarian, kosher, or gluten-free options" ;
              rdfs:label "Special_Meal" .


###  http://www.semanticweb.org/kiki/ontologies/2024/3/Global_Airline_Satisfaction_Framework#Standard_Meal
:Standard_Meal rdf:type owl:Class ;
               rdfs:subClassOf :Meal_Service ;
               rdfs:comment "The regular meal provided to passengers, which varies depending on the airline and class." ;
               rdfs:label "Standard_Meal" .


###  http://www.semanticweb.org/kiki/ontologies/2024/3/Global_Airline_Satisfaction_Framework#Technical_Training
:Technical_Training rdf:type owl:Class ;
                    rdfs:subClassOf :Crew_Training ;
                    rdfs:comment "Training that provides technical knowledge necessary for operating and maintaining aircraft systems" ;
                    rdfs:label "Technical_Training" .


###  http://www.semanticweb.org/kiki/ontologies/2024/3/Global_Airline_Satisfaction_Framework#Terminal_Facilities
:Terminal_Facilities rdf:type owl:Class ;
                     rdfs:subClassOf :Airport_Infrastructure ;
                     rdfs:comment "Facilities within airport terminals that enhance passenger comfort and provide necessary services." ;
                     rdfs:label "Terminal_Facilities" .


###  http://www.semanticweb.org/kiki/ontologies/2024/3/Global_Airline_Satisfaction_Framework#Tier_Levels
:Tier_Levels rdf:type owl:Class ;
             rdfs:subClassOf :Loyalty_Rewards ;
             rdfs:comment "Different levels within a loyalty program that offer increasing benefits." ;
             rdfs:label "Tier_Levels" .


###  http://www.semanticweb.org/kiki/ontologies/2024/3/Global_Airline_Satisfaction_Framework#Travel_Class
:Travel_Class rdf:type owl:Class ;
              rdfs:subClassOf :Loyalty_Rewards ;
              rdfs:comment "Represents different classes of service offered by airlines, each providing varying levels of amenities and space." ;
              rdfs:label "Travel_Class" .


###  http://www.semanticweb.org/kiki/ontologies/2024/3/Global_Airline_Satisfaction_Framework#Waste_Reduction_Initiatives
:Waste_Reduction_Initiatives rdf:type owl:Class ;
                             rdfs:subClassOf :Environmental_Impact ;
                             rdfs:comment "Efforts to minimize waste generated during flights through recycling and sustainable practices" ;
                             rdfs:label "Waste_Reduction_Initiatives" .


#################################################################
#    Individuals
#################################################################

###  http://www.semanticweb.org/kiki/ontologies/2024/3/Global_Airline_Satisfaction_Framework#CityAirport
:CityAirport rdf:type owl:NamedIndividual ,
                      :Airport ;
             :location "Los Angeles" ;
             :sameAs "http://dbpedia.org/resource/Heathrow_Airport" ;
             rdfs:comment "Main airport located in the metropolitan area of the city." ;
             rdfs:label "City Airport" .


###  http://www.semanticweb.org/kiki/ontologies/2024/3/Global_Airline_Satisfaction_Framework#ExampleAirline
:ExampleAirline rdf:type owl:NamedIndividual ,
                         :Airline ;
                :name "qatar" ;
                rdfs:comment "A leading airline offering global flight services." ;
                rdfs:label "Example Airline" .


###  http://www.semanticweb.org/kiki/ontologies/2024/3/Global_Airline_Satisfaction_Framework#FlexibleRebooking
:FlexibleRebooking rdf:type owl:NamedIndividual ,
                            :Airline_Policies ;
                   :policyDescription "Allows rebooking with no extra charge" ;
                   rdfs:comment "Allows passengers to rebook their flights without any additional charges under certain conditions" ;
                   rdfs:label "Flexible Rebooking Policy" .


###  http://www.semanticweb.org/kiki/ontologies/2024/3/Global_Airline_Satisfaction_Framework#InFlightMeal
:InFlightMeal rdf:type owl:NamedIndividual ,
                       :Service ;
              rdfs:comment "Provides meal services for passengers during flights." ;
              rdfs:label "In-Flight Meal Service" .


###  http://www.semanticweb.org/kiki/ontologies/2024/3/Global_Airline_Satisfaction_Framework#PepePassenger
:PepePassenger rdf:type owl:NamedIndividual ,
                        :Passenger ;
               :locatedAtAirport :ExampleAirline ;
               :email "pepe@gmail.com" ;
               rdfs:comment "A frequent flyer with Example Airline." ;
               rdfs:label "pepe" .


#################################################################
#    Rules
#################################################################

<http://www.semanticweb.org/kiki/ontologies/2024/3/Global_Airline_Satisfaction_Framework/f> rdf:type <http://www.w3.org/2003/11/swrl#Variable> .

<http://www.semanticweb.org/kiki/ontologies/2024/3/Global_Airline_Satisfaction_Framework/p> rdf:type <http://www.w3.org/2003/11/swrl#Variable> .

<http://www.semanticweb.org/kiki/ontologies/2024/3/Global_Airline_Satisfaction_Framework/points> rdf:type <http://www.w3.org/2003/11/swrl#Variable> .

<http://www.semanticweb.org/kiki/ontologies/2024/3/Global_Airline_Satisfaction_Framework/rating> rdf:type <http://www.w3.org/2003/11/swrl#Variable> .

[ <http://swrl.stanford.edu/ontologies/3.3/swrla.owl#isRuleEnabled> "true"^^xsd:boolean ;
   rdfs:comment "" ;
   rdfs:label "S1" ;
   rdf:type <http://www.w3.org/2003/11/swrl#Imp> ;
   <http://www.w3.org/2003/11/swrl#body> [ rdf:type <http://www.w3.org/2003/11/swrl#AtomList> ;
                                           rdf:first [ rdf:type <http://www.w3.org/2003/11/swrl#ClassAtom> ;
                                                       <http://www.w3.org/2003/11/swrl#classPredicate> :Passenger ;
                                                       <http://www.w3.org/2003/11/swrl#argument1> <http://www.semanticweb.org/kiki/ontologies/2024/3/Global_Airline_Satisfaction_Framework/p>
                                                     ] ;
                                           rdf:rest [ rdf:type <http://www.w3.org/2003/11/swrl#AtomList> ;
                                                      rdf:first [ rdf:type <http://www.w3.org/2003/11/swrl#IndividualPropertyAtom> ;
                                                                  <http://www.w3.org/2003/11/swrl#propertyPredicate> :hasLoyaltyPoints ;
                                                                  <http://www.w3.org/2003/11/swrl#argument1> <http://www.semanticweb.org/kiki/ontologies/2024/3/Global_Airline_Satisfaction_Framework/p> ;
                                                                  <http://www.w3.org/2003/11/swrl#argument2> <http://www.semanticweb.org/kiki/ontologies/2024/3/Global_Airline_Satisfaction_Framework/points>
                                                                ] ;
                                                      rdf:rest [ rdf:type <http://www.w3.org/2003/11/swrl#AtomList> ;
                                                                 rdf:first [ rdf:type <http://www.w3.org/2003/11/swrl#BuiltinAtom> ;
                                                                             <http://www.w3.org/2003/11/swrl#builtin> <http://www.w3.org/2003/11/swrlb#greaterThan> ;
                                                                             <http://www.w3.org/2003/11/swrl#arguments> [ rdf:type rdf:List ;
                                                                                                                          rdf:first <http://www.semanticweb.org/kiki/ontologies/2024/3/Global_Airline_Satisfaction_Framework/points> ;
                                                                                                                          rdf:rest [ rdf:type rdf:List ;
                                                                                                                                     rdf:first 1000 ;
                                                                                                                                     rdf:rest rdf:nil
                                                                                                                                   ]
                                                                                                                        ]
                                                                           ] ;
                                                                 rdf:rest rdf:nil
                                                               ]
                                                    ]
                                         ] ;
   <http://www.w3.org/2003/11/swrl#head> [ rdf:type <http://www.w3.org/2003/11/swrl#AtomList> ;
                                           rdf:first [ rdf:type <http://www.w3.org/2003/11/swrl#DatavaluedPropertyAtom> ;
                                                       <http://www.w3.org/2003/11/swrl#propertyPredicate> :hasBoardingStatus ;
                                                       <http://www.w3.org/2003/11/swrl#argument1> <http://www.semanticweb.org/kiki/ontologies/2024/3/Global_Airline_Satisfaction_Framework/p> ;
                                                       <http://www.w3.org/2003/11/swrl#argument2> "Priority"
                                                     ] ;
                                           rdf:rest rdf:nil
                                         ]
 ] .

[ <http://swrl.stanford.edu/ontologies/3.3/swrla.owl#isRuleEnabled> "true"^^xsd:boolean ;
   rdfs:comment "" ;
   rdfs:label "S3" ;
   rdf:type <http://www.w3.org/2003/11/swrl#Imp> ;
   <http://www.w3.org/2003/11/swrl#body> [ rdf:type <http://www.w3.org/2003/11/swrl#AtomList> ;
                                           rdf:first [ rdf:type <http://www.w3.org/2003/11/swrl#ClassAtom> ;
                                                       <http://www.w3.org/2003/11/swrl#classPredicate> :Passenger ;
                                                       <http://www.w3.org/2003/11/swrl#argument1> <http://www.semanticweb.org/kiki/ontologies/2024/3/Global_Airline_Satisfaction_Framework/p>
                                                     ] ;
                                           rdf:rest [ rdf:type <http://www.w3.org/2003/11/swrl#AtomList> ;
                                                      rdf:first [ rdf:type <http://www.w3.org/2003/11/swrl#DatavaluedPropertyAtom> ;
                                                                  <http://www.w3.org/2003/11/swrl#propertyPredicate> :hasSatisfactionRating ;
                                                                  <http://www.w3.org/2003/11/swrl#argument1> <http://www.semanticweb.org/kiki/ontologies/2024/3/Global_Airline_Satisfaction_Framework/p> ;
                                                                  <http://www.w3.org/2003/11/swrl#argument2> <http://www.semanticweb.org/kiki/ontologies/2024/3/Global_Airline_Satisfaction_Framework/rating>
                                                                ] ;
                                                      rdf:rest [ rdf:type <http://www.w3.org/2003/11/swrl#AtomList> ;
                                                                 rdf:first [ rdf:type <http://www.w3.org/2003/11/swrl#BuiltinAtom> ;
                                                                             <http://www.w3.org/2003/11/swrl#builtin> <http://www.w3.org/2003/11/swrlb#lessThan> ;
                                                                             <http://www.w3.org/2003/11/swrl#arguments> [ rdf:type rdf:List ;
                                                                                                                          rdf:first <http://www.semanticweb.org/kiki/ontologies/2024/3/Global_Airline_Satisfaction_Framework/rating> ;
                                                                                                                          rdf:rest [ rdf:type rdf:List ;
                                                                                                                                     rdf:first 3 ;
                                                                                                                                     rdf:rest rdf:nil
                                                                                                                                   ]
                                                                                                                        ]
                                                                           ] ;
                                                                 rdf:rest rdf:nil
                                                               ]
                                                    ]
                                         ] ;
   <http://www.w3.org/2003/11/swrl#head> [ rdf:type <http://www.w3.org/2003/11/swrl#AtomList> ;
                                           rdf:first [ rdf:type <http://www.w3.org/2003/11/swrl#DatavaluedPropertyAtom> ;
                                                       <http://www.w3.org/2003/11/swrl#propertyPredicate> :offeredDiscount ;
                                                       <http://www.w3.org/2003/11/swrl#argument1> <http://www.semanticweb.org/kiki/ontologies/2024/3/Global_Airline_Satisfaction_Framework/p> ;
                                                       <http://www.w3.org/2003/11/swrl#argument2> "true"^^xsd:boolean
                                                     ] ;
                                           rdf:rest rdf:nil
                                         ]
 ] .

[ <http://swrl.stanford.edu/ontologies/3.3/swrla.owl#isRuleEnabled> "true"^^xsd:boolean ;
   rdfs:comment "" ;
   rdfs:label "S2" ;
   rdf:type <http://www.w3.org/2003/11/swrl#Imp> ;
   <http://www.w3.org/2003/11/swrl#body> [ rdf:type <http://www.w3.org/2003/11/swrl#AtomList> ;
                                           rdf:first [ rdf:type <http://www.w3.org/2003/11/swrl#ClassAtom> ;
                                                       <http://www.w3.org/2003/11/swrl#classPredicate> :Flight_Schedule ;
                                                       <http://www.w3.org/2003/11/swrl#argument1> <http://www.semanticweb.org/kiki/ontologies/2024/3/Global_Airline_Satisfaction_Framework/f>
                                                     ] ;
                                           rdf:rest [ rdf:type <http://www.w3.org/2003/11/swrl#AtomList> ;
                                                      rdf:first [ rdf:type <http://www.w3.org/2003/11/swrl#DatavaluedPropertyAtom> ;
                                                                  <http://www.w3.org/2003/11/swrl#propertyPredicate> :isDelayed ;
                                                                  <http://www.w3.org/2003/11/swrl#argument1> <http://www.semanticweb.org/kiki/ontologies/2024/3/Global_Airline_Satisfaction_Framework/f> ;
                                                                  <http://www.w3.org/2003/11/swrl#argument2> "true"^^xsd:boolean
                                                                ] ;
                                                      rdf:rest [ rdf:type <http://www.w3.org/2003/11/swrl#AtomList> ;
                                                                 rdf:first [ rdf:type <http://www.w3.org/2003/11/swrl#DatavaluedPropertyAtom> ;
                                                                             <http://www.w3.org/2003/11/swrl#propertyPredicate> :bookedOnFlight ;
                                                                             <http://www.w3.org/2003/11/swrl#argument1> <http://www.semanticweb.org/kiki/ontologies/2024/3/Global_Airline_Satisfaction_Framework/p> ;
                                                                             <http://www.w3.org/2003/11/swrl#argument2> <http://www.semanticweb.org/kiki/ontologies/2024/3/Global_Airline_Satisfaction_Framework/f>
                                                                           ] ;
                                                                 rdf:rest rdf:nil
                                                               ]
                                                    ]
                                         ] ;
   <http://www.w3.org/2003/11/swrl#head> [ rdf:type <http://www.w3.org/2003/11/swrl#AtomList> ;
                                           rdf:first [ rdf:type <http://www.w3.org/2003/11/swrl#DatavaluedPropertyAtom> ;
                                                       <http://www.w3.org/2003/11/swrl#propertyPredicate> :isNotifiedOfDelay ;
                                                       <http://www.w3.org/2003/11/swrl#argument1> <http://www.semanticweb.org/kiki/ontologies/2024/3/Global_Airline_Satisfaction_Framework/p> ;
                                                       <http://www.w3.org/2003/11/swrl#argument2> "true"^^xsd:boolean
                                                     ] ;
                                           rdf:rest rdf:nil
                                         ]
 ] .

###  Generated by the OWL API (version 5.1.18) https://github.com/owlcs/owlapi/
